fairneris/aneris_lang/network_model.v
@@ -1,0 +1,77 @@
+From trillium.prelude Require Export finitary quantifiers sigma classical_instances.
+From fairneris Require Export trace_utils fairness env_model.
+From fairneris.aneris_lang Require Import ast network lang aneris_lang.
+
+
+Definition net_state : Set :=
+  message_multi_soup * gmap socket_address (list message).
+
+Inductive net_trans : net_state → (action aneris_lang + config_label aneris_lang) → net_state → Prop :=
+| NetSend ms bs msg :
+  net_trans (ms, bs) (inl $ Send msg) (ms ⊎ {[+ msg +]}, bs)
+| NetDuplicate ms bs msg :
+  msg ∈ ms → net_trans (ms, bs) (inr $ Duplicate msg) (ms ⊎ {[+ msg +]}, bs)
+| NetDrop ms bs msg :
+  msg ∈ ms →
+  net_trans (ms, bs) (inr (Drop msg)) (ms ∖ {[+ msg +]}, bs)
+| NetDeliver ms ms' bs msg :
+  msg ∈ ms →
+  bs !!! m_destination msg = ms' →
+  net_trans (ms, bs) (inr (Deliver msg)) (ms ∖ {[+ msg +]}, <[m_destination msg := msg::ms']>bs)
+| NetRecvFail ms bs sa :
+  bs !!! sa = [] →
+  net_trans (ms, bs) (inl $ (Recv None)) (ms, bs)
+| NetRecvSucc ms bs msg ms' sa :
+  bs !!! sa = ms'++[msg] →
+  net_trans (ms, bs) (inl $ Recv (Some msg)) (ms, <[sa := ms']>bs).
+
+Program Definition net_lts : Lts (action aneris_lang + config_label aneris_lang) :=
+  {|
+    lts_state := net_state;
+    lts_trans := net_trans;
+  |}.
+
+Record Lts lab `{Countable lab, Inhabited lab}: Type := {
+  lts_state :> Type;
+  lts_state_eqdec :: EqDecision lts_state;
+  lts_state_inhabited :: Inhabited lts_state;
+
+  lts_trans: lts_state → lab → lts_state → Prop;
+}.
+
+Definition model_state_socket_coh
+           (skts : gmap ip_address sockets)
+           (bs : gmap socket_address (list message)) :=
+  ∀ ip Sn sh skt sa ms,
+  skts !! ip = Some Sn → Sn !! sh = Some (skt,ms) →
+  saddress skt = Some sa →
+  bs !!! sa = ms.
+
+Definition config_net_match (c : cfg aneris_lang) (δ : net_state) :=
+  state_ms c.2 = δ.1 ∧ model_state_socket_coh (state_sockets c.2) δ.2.
+
+Definition net_apply_trans (s: net_state) (l: action aneris_lang + config_label aneris_lang) : net_state :=
+  let '(ms, bs) := s in
+  match l with
+  | inl (Send msg) => (ms ⊎ {[+ msg +]}, bs)
+  | inr (Duplicate msg) => (ms ⊎ {[+ msg +]}, bs)
+  | inr (Drop msg) => (ms ∖ {[+ msg +]}, bs)
+  | inr (Deliver msg) =>
+      let ms' := bs !!! m_destination msg in
+      (ms ∖ {[+ msg +]}, <[m_destination msg := msg::ms']>bs)
+  | inl (Recv None) => (ms, bs)
+  | inl (Recv (Some msg)) =>
+      let ms' := bs !!! m_destination msg in
+      (ms, <[m_destination msg := take (length ms' - 1) ms']>bs)
+  end.
+
+Program Definition net_model : EnvModel aneris_lang :=
+  {|
+    env_lts := net_lts;
+    env_states_match := config_net_match;
+    env_apply_trans := net_apply_trans;
+    env_fairness _ := True;
+  |}.
+Next Obligation.
+  (* Correctness of [net_apply_trans] *)
+Admitted.
