fairneris/env_model.v
@@ -1,59 +1,63 @@
 From stdpp Require Import option countable.
 From fairneris Require Export inftraces trace_utils fairness.
 
-Record Lts lab : Type := {
+Record Lts lab `{Countable lab, Inhabited lab}: Type := {
   lts_state :> Type;
   lts_state_eqdec :: EqDecision lts_state;
   lts_state_inhabited :: Inhabited lts_state;
 
-  lts_lab_eqdec :: EqDecision lab;
-  lts_lab_countable : Countable lab;
-  lts_lab_inhabited :: Inhabited lab;
-
   lts_trans: lts_state → lab → lts_state → Prop;
 }.
 
-Arguments lts_state {_}.
-Arguments lts_trans {_}.
+Arguments lts_state {_ _ _ _}.
+Arguments lts_trans {_ _ _ _}.
 
-Record EnvModel (Λ : language) := {
+Section models.
+  Context (Λ: language).
+  Context `{Countable (config_label Λ)}.
+  Context `{Countable (action Λ)}.
+  Context `{Inhabited (config_label Λ)}.
+  Context `{Inhabited (action Λ)}.
+
+Record EnvModel := {
     env_lts :> Lts (action Λ + config_label Λ);
     env_states_match : cfg Λ → env_lts.(lts_state) → Prop;
-    env_apply_trans : env_lts.(lts_state) → config_label Λ → env_lts.(lts_state);
-    env_apply_trans_spec : ∀ c1 m1 cl c2 m2,
+    env_apply_trans : env_lts.(lts_state) → (action Λ + config_label Λ) → env_lts.(lts_state);
+    env_apply_trans_spec_both : ∀ ζ c1 m1 cl c2 m2,
       env_apply_trans m1 cl = m2 →
-      locale_step c1 (inr cl) c2 →
+      locale_step c1 (sum_map (λ α, (ζ, Some α)) id cl) c2 →
       env_states_match c1 m1 →
       env_states_match c2 m2;
+    env_fairness: trace env_lts.(lts_state) (action Λ + config_label Λ) → Prop;
 }.
 
 Arguments env_lts {_}.
 
-Record UserModel (Λ : language) := {
+Record UserModel := {
     usr_role : Type;
+
+    usr_eqdec:: EqDecision usr_role;
+    usr_countable:: Countable usr_role;
+    usr_inhabited:: Inhabited usr_role;
+
     usr_lts :> Lts (usr_role * option (action Λ));
 
-    usr_eqdec: EqDecision usr_role;
-    usr_countable: Countable usr_role;
-    usr_inhabited: Inhabited usr_role;
     usr_live_roles: usr_lts.(lts_state) → gset usr_role;
     usr_live_spec: ∀ s ρ α s', usr_lts.(lts_trans) s (ρ,α) s' → ρ ∈ usr_live_roles s;
 }.
 
-Arguments usr_role {_}.
-Arguments usr_lts {_}.
-Arguments usr_live_roles {_ _}.
+Arguments usr_live_roles {_}.
 
-Inductive joint_trans {Λ: language} {M: UserModel Λ} {N: EnvModel Λ} :
+Inductive joint_trans {M: UserModel} {N: EnvModel} :
   (M * N) → ((usr_role M * option (action Λ)) + config_label Λ) → (M * N) → Prop :=
 | UsrTrans n u1 u2 ρ : lts_trans M u1 (ρ, None) u2 → joint_trans (u1, n) (inl (ρ, None)) (u2, n)
 | NetTrans u n1 n2 ℓ : lts_trans N n1 (inr ℓ) n2 → joint_trans (u, n2) (inr ℓ) (u, n2)
 | SyncTrans u1 u2 n1 n2 ρ α :
   lts_trans M u1 (ρ, Some α) u2 → lts_trans N n1 (inl α) n2 →
-  joint_trans (u1, n2) (inl (ρ, Some α)) (u2, n2)
+  joint_trans (u1, n1) (inl (ρ, Some α)) (u2, n2)
 .
 
-Program Definition joint_model {Λ: language} (M: UserModel Λ) (N: EnvModel Λ) : FairModel :=
+Program Definition joint_model (M: UserModel) (N: EnvModel) : FairModel :=
 {|
   fmstate := lts_state (usr_lts M) * lts_state N;
   (* Why doesn't this work??? *)
@@ -63,11 +67,12 @@ Program Definition joint_model {Λ: language} (M: UserModel Λ) (N: EnvModel Λ)
   fmtrans s1 ℓ s2 := joint_trans s1 ℓ s2;
   live_roles s := usr_live_roles s.1;
 
-  fmrole_eqdec := usr_eqdec _ M;
-  fmrole_countable := usr_countable _ M;
-  fmrole_inhabited := usr_inhabited _ M;
-
-  (* let's see what to do later... *)
+  (* We want somehting like: *)
+  (* fmfairness tr := env_fairness _ tr; *)
+  (* but it's not so easy, because this definition is not constructive... *)
+  (* it may be easier to only state it on the joint model directly... *)
   fmfairness _ := True;
 |}.
-Next Obligation. by intros ???????; inversion 1; simplify_eq; eapply usr_live_spec. Qed.
+Next Obligation. by intros ??????; inversion 1; simplify_eq; eapply usr_live_spec. Qed.
+
+End models.
